Using the identities

\begin{align*}
    sn(u+v)&={\frac {sn \left( u \right) cn \left( v \right) dn
 \left( v \right) +sn \left( v \right) cn \left( u
 \right) dn \left( u \right) }{\Delta \left( u,v \right) }}
\\
cn(u+v)&={\frac {cn \left( u \right) cn \left( v \right) -sn
 \left( u \right) sn \left( v \right) dn \left( u \right) 
dn \left( v \right) }{\Delta \left( u,v \right) }}
\\
dn(u+v)&={\frac {dn \left( u \right) dn \left( v \right) -{k}^{2}{
\it sn} \left( u \right) sn \left( v \right) cn \left( u
 \right) cn \left( v \right) }{\Delta \left( u,v \right) }}\\
\Delta(u,v)&=1-k^2 sn^2u\, sn^2v,\;\;\;  dn^2(u)+k^2sn^2(u)=1
\end{align*}
It follows that 

\[L_\pm(u)=L_\pm(0)=2 \,cn(\sigma)
sn(\sigma) \frac{\sqrt{ \delta_{\pm}R}}{k} \sum_{j=1}^{N}
  \,\frac{
  dn^2(j \sigma) }{  1-   \left(1-  dn^{2}(j \sigma) \right) 
  sn^{2}(\sigma)}
\]

\noindent where as before $\sigma=(4 \tau K)/N$.






