Consider the pair of nested circles:
 
\[\C_{int}:\;x^2+y^2=r^2,\;\;\;\C_{ext}:\;(x+d)^2+y^2=R^2\]
Their limiting points $\ell_1$ and $\ell_2$ are given by \cite[Limiting Points]{mw}:
 
 \[ \ell_1= (R^2 - d^2 - r^2 -\Delta)/(2d),\;\;\;\ell_2=(R^2 - d^2 - r^2 + \Delta)/(2 d)\]
where:
 \[ \Delta=\sqrt { \left( d+R+r \right)  \left( R-d+r \right)  \left( R+d-r
 \right)  \left( R-d-r \right) }\]

Notice $\ell_1$ (resp. $\ell_2$) is internal (resp. external) to the circle pair. Below we show that the polar image of the  $\C_{int},\C_{ext}$ pair with respect to a circle of radius $\rho$ centered on $\ell_1$ (resp. $\ell_2$) is a confocal pair of ellipses (resp. hyperbolas).

\begin{lemma}
The polar image of $\C_{int}$ with respect to $\ell_1 $ is the ellipse $\E$ centered at
 \[ \O_e=\left[  {\rho}^2\frac{d}{\Delta} +\frac{k-\Delta}{2d},0\right] \]
where $k=R^2 - d^2 - r^2$. Its semi-axes are given by:
 
\[  a^2={\rho}^4\left(\frac{2d^2r^2+ \Delta(k+\Delta)}{ 2 \Delta^2 r^2}\right),\;\;\;b^2= {\rho}^4\left(\frac{k+ \Delta}{2 \Delta r^2}\right) \]
 \end{lemma}
\noindent Note that $c^2=a^2-b^2={\rho}^4d^2/{\Delta^2}$.
 
 \begin{lemma}
 The polar image of $\C_{ext}$ with respect to $\ell_1$ is an ellipse $\E'$ confocal with $\E$ with semi-axes given by:
 
\[  a'^2= {\rho}^4\frac{(2R^2d^2 + \Delta (k'+\Delta ))}{ 2 \Delta^2 R^2},\;\;\;b'^2=  {\rho}^4\left(\frac{k'+\Delta}{ 2 \Delta R^2}\right) \]
 \end{lemma}
 \noindent where $k'=R^2 + d^2 - r^2$.
 
 \begin{lemma}
 The polar image of $\C_{int}$ with respect to $\ell_2 $ is the hyperbola $\H$ centered at
  \[  \O_h=\left[  {-\rho}^2\frac{d}{\Delta} +\frac{k+\Delta}{2d},0\right] \]
 with semiaxes given by:
 
\[  a_h^2={\rho}^4\left(\frac{  2d^2r^2-\Delta(k - \Delta)}{2  \Delta^2 r^2}\right),\;\;\;b_h^2= {\rho}^4\left(\frac{k - \Delta}{2 \Delta r^2}\right)\]
 \end{lemma}
 \noindent Note that $c_h^2=a_h^2+b_h^2={{\rho}^4d^2}/{\Delta^2}$. Note also that $c=c_h$.
 
 \begin{lemma} The polar image of $\C_{out}$ with respect to $\ell_2$ is a hyperbola $\H'$ confocal with $\H$. Its semiaxes are given by:
 
\[ a_h'^2= {\rho}^4\left(\frac{2R^2d^2 - \Delta (k' - \Delta)}{ 2 \Delta^2 R^2}\right),\;\;\; b_h'^2= {\rho}^4 \left(\frac{k' - \Delta}{ 2 \Delta R^2}\right)\]
 \end{lemma}


